transformations/Moore2Mealy/Moore.v
@@ -221,6 +221,87 @@ Definition Transition_getTargetObject (tr_arg : Transition_t) (m : M) : option (
   end. (* option_map *)
 
 
+Lemma In_state : forall (m:Moore.M) e,
+         List.In (StateElement e) (Model.modelElements m) <-> List.In e
+    (OptionListUtils.lift_list (get_E_data State_K)
+       (Model.modelElements m)).
+Proof.
+  intros m e.
+  split ; intro H.
+  {
+    apply OptionListUtils.In_lift.
+    exists (StateElement e). auto.
+  }  
+  {
+    apply OptionListUtils.In_lift in H.
+    destruct H as (e2 & (G & IN2)).
+    destruct e2 ; [ PropUtils.inj G| discriminate G]. 
+    assumption.
+  }
+Qed.
+
+
+Lemma In_transition : forall (m:Moore.M) e,
+         List.In (TransitionElement e) (Model.modelElements m) <-> List.In e
+    (OptionListUtils.lift_list (get_E_data Transition_K)
+       (Model.modelElements m)).
+Proof.
+  intros m e.
+  split ; intro H.
+  {
+    apply OptionListUtils.In_lift.
+    exists (TransitionElement e). auto.
+  }  
+  {
+    apply OptionListUtils.In_lift in H.
+    destruct H as (e2 & (G & IN2)).
+    destruct e2 ; [ discriminate G | PropUtils.inj G]. 
+    assumption.
+  }
+Qed.
+
+
+Lemma In_transition_sourceLink : 
+  forall (m:Moore.M) e,
+         List.In (Transition_sourceLink e) (Model.modelLinks m) <-> List.In e
+    (OptionListUtils.lift_list (get_L_data Transition_source_K)
+       (Model.modelLinks m)).
+Proof.
+  intros m e.
+  split ; intro H.
+  {
+    apply OptionListUtils.In_lift.
+    exists (Transition_sourceLink e). auto.
+  }  
+  {
+    apply OptionListUtils.In_lift in H.
+    destruct H as (e2 & (G & IN2)).
+    destruct e2 ; [ PropUtils.inj G | discriminate G]. 
+    assumption.
+  }
+Qed.
+
+Lemma In_transition_targetLink : 
+  forall (m:Moore.M) e,
+         List.In (Transition_targetLink e) (Model.modelLinks m) <-> List.In e
+    (OptionListUtils.lift_list (get_L_data Transition_target_K)
+       (Model.modelLinks m)).
+Proof.
+  intros m e.
+  split ; intro H.
+  {
+    apply OptionListUtils.In_lift.
+    exists (Transition_targetLink e). auto.
+  }  
+  {
+    apply OptionListUtils.In_lift in H.
+    destruct H as (e2 & (G & IN2)).
+    destruct e2 ; [ discriminate G | PropUtils.inj G]. 
+    assumption.
+  }
+Qed.
+
+
 Lemma getTransition_source_inv m t s : 
   getTransition_source m t = Some s ->
   let lk := {|  Transition_source_t_source := t ;  Transition_source_t_target := s |} in
